testdata/cue/builtins/aliased_list_const.cue
@@ -1,0 +1,5 @@
+import l "list"
+
+asc: l.Sort([3, 1, 2], l.Ascending)
+desc: l.Sort([3, 1, 2], l.Descending)
+cmp: l.Comparer
